@prefix base: <https://w3id.org/earthsemantics/ODATIS/thesaurus> .
@prefix dc: <http://purl.org/dc/elements/1.1/> .
@prefix dcterms: <http://purl.org/dc/terms/> .
@prefix ns1: <http://www.isotc211.org/schemas/grg/> .
@prefix ns2: <http://purl.org/pav/> .
@prefix owl: <http://www.w3.org/2002/07/owl#> .
@prefix rdfs: <http://www.w3.org/2000/01/rdf-schema#> .
@prefix skos: <http://www.w3.org/2004/02/skos/core#> .
@prefix void: <http://rdfs.org/ns/void#> .

<http://vocab.nerc.ac.uk/collection/OD1/current/> a skos:Collection ;
    dcterms:alternative "ODATIS APG and EV" ;
    dcterms:creator "ODATIS vocabulary governance" ;
    dcterms:date "2024-06-07 03:00:04.0" ;
    dcterms:description "Collection of terms used within the French Ocean Data and Services Cluster ODATIS for data discovery and product or dataset aggregation. Whenever applicable, Essential Variable terms are linked to the authoritative source of Essential Climate Ocean and Biodiversity Variable definitions maintained by the Global Observing System for Climate (GCOS), the Global Ocean Observing System (GOOS) and the Group on Earth Observations Biodiversity Observation Network (GEO BON)." ;
    dcterms:publisher "Natural Environment Research Council" ;
    dcterms:title "ODATIS aggregation parameters and Essential Variable names" ;
    ns1:RE_RegisterManager "British Oceanographic Data Centre" ;
    ns1:RE_RegisterOwner "ODATIS vocabulary governance" ;
    rdfs:comment "Governance for vocabularies used in the ODATIS Ocean Data and Services Cluster of the French Data Terra Research Infrastructure and hosted on the NVS." ;
    owl:versionInfo "8" ;
    skos:altLabel "ODATIS APG and EV" ;
    skos:member <http://vocab.nerc.ac.uk/collection/OD1/current/ACOUST/>,
        <http://vocab.nerc.ac.uk/collection/OD1/current/AERO/>,
        <http://vocab.nerc.ac.uk/collection/OD1/current/AIRPRES/>,
        <http://vocab.nerc.ac.uk/collection/OD1/current/AIRTEMP/>,
        <http://vocab.nerc.ac.uk/collection/OD1/current/BATHY/>,
        <http://vocab.nerc.ac.uk/collection/OD1/current/BENTHA/>,
        <http://vocab.nerc.ac.uk/collection/OD1/current/BIOINFO/>,
        <http://vocab.nerc.ac.uk/collection/OD1/current/BIOTOX/>,
        <http://vocab.nerc.ac.uk/collection/OD1/current/C02/>,
        <http://vocab.nerc.ac.uk/collection/OD1/current/COLOUR/>,
        <http://vocab.nerc.ac.uk/collection/OD1/current/CONT/>,
        <http://vocab.nerc.ac.uk/collection/OD1/current/CURR/>,
        <http://vocab.nerc.ac.uk/collection/OD1/current/DENS/>,
        <http://vocab.nerc.ac.uk/collection/OD1/current/DOM/>,
        <http://vocab.nerc.ac.uk/collection/OD1/current/DOXY/>,
        <http://vocab.nerc.ac.uk/collection/OD1/current/FISH/>,
        <http://vocab.nerc.ac.uk/collection/OD1/current/FLUO/>,
        <http://vocab.nerc.ac.uk/collection/OD1/current/GEOL/>,
        <http://vocab.nerc.ac.uk/collection/OD1/current/HCORAL/>,
        <http://vocab.nerc.ac.uk/collection/OD1/current/HEATCON/>,
        <http://vocab.nerc.ac.uk/collection/OD1/current/HUMACT/>,
        <http://vocab.nerc.ac.uk/collection/OD1/current/HUMI/>,
        <http://vocab.nerc.ac.uk/collection/OD1/current/INVER/>,
        <http://vocab.nerc.ac.uk/collection/OD1/current/MACALG/>,
        <http://vocab.nerc.ac.uk/collection/OD1/current/MANG/>,
        <http://vocab.nerc.ac.uk/collection/OD1/current/MTBM/>,
        <http://vocab.nerc.ac.uk/collection/OD1/current/N2O/>,
        <http://vocab.nerc.ac.uk/collection/OD1/current/NUTS/>,
        <http://vocab.nerc.ac.uk/collection/OD1/current/PATHOGEN/>,
        <http://vocab.nerc.ac.uk/collection/OD1/current/PHYTO/>,
        <http://vocab.nerc.ac.uk/collection/OD1/current/PIGM/>,
        <http://vocab.nerc.ac.uk/collection/OD1/current/PRESS/>,
        <http://vocab.nerc.ac.uk/collection/OD1/current/RADFLX/>,
        <http://vocab.nerc.ac.uk/collection/OD1/current/RAIN/>,
        <http://vocab.nerc.ac.uk/collection/OD1/current/SAL/>,
        <http://vocab.nerc.ac.uk/collection/OD1/current/SEAICE/>,
        <http://vocab.nerc.ac.uk/collection/OD1/current/SEALVL/>,
        <http://vocab.nerc.ac.uk/collection/OD1/current/SEATEMP/>,
        <http://vocab.nerc.ac.uk/collection/OD1/current/SEDFLUX/>,
        <http://vocab.nerc.ac.uk/collection/OD1/current/SEISM/>,
        <http://vocab.nerc.ac.uk/collection/OD1/current/SGRAS/>,
        <http://vocab.nerc.ac.uk/collection/OD1/current/SHORE/>,
        <http://vocab.nerc.ac.uk/collection/OD1/current/SUSPMA/>,
        <http://vocab.nerc.ac.uk/collection/OD1/current/TIDES/>,
        <http://vocab.nerc.ac.uk/collection/OD1/current/TRACELE/>,
        <http://vocab.nerc.ac.uk/collection/OD1/current/TRANST/>,
        <http://vocab.nerc.ac.uk/collection/OD1/current/TURBID/>,
        <http://vocab.nerc.ac.uk/collection/OD1/current/WAVES/>,
        <http://vocab.nerc.ac.uk/collection/OD1/current/WIND/>,
        <http://vocab.nerc.ac.uk/collection/OD1/current/ZOO/> ;
    skos:prefLabel "ODATIS aggregation parameters and Essential Variable names" .

<https://vocab.ifremer.fr/scheme/SXT/IR/145aed26-0b02-4d37-9d24-8db12fa0967e> skos:broader <https://w3id.org/earthsemantics/ODATIS/IR> ;
    skos:inScheme base: .

<https://vocab.ifremer.fr/scheme/SXT/IR/3c3341a0-6b6b-4184-bada-671a1dbb53bc> skos:broader <https://w3id.org/earthsemantics/ODATIS/IR> ;
    skos:inScheme base: .

<https://vocab.ifremer.fr/scheme/SXT/IR/78d02f74-443a-4010-a9d2-af54f183cea0> skos:broader <https://w3id.org/earthsemantics/ODATIS/IR> ;
    skos:inScheme base: .

<https://vocab.ifremer.fr/scheme/SXT/IR/afae62c5-9962-4850-b174-f4edd6caf3c3> skos:broader <https://w3id.org/earthsemantics/ODATIS/IR> ;
    skos:inScheme base: .

<https://vocab.ifremer.fr/scheme/SXT/IR/cb34cf11-5fe5-425b-b5ed-7a5c1a5f842e> skos:broader <https://w3id.org/earthsemantics/ODATIS/IR> ;
    skos:inScheme base: .

<https://vocab.ifremer.fr/scheme/SXT/SNO/064702d0-17d7-40dd-8f6e-e3421a71ce7c> skos:broader <https://w3id.org/earthsemantics/ODATIS/SNO> ;
    skos:inScheme base: .

<https://vocab.ifremer.fr/scheme/SXT/SNO/11b798fe-169e-4bc7-bb34-44823e874adb> skos:broader <https://w3id.org/earthsemantics/ODATIS/SNO> ;
    skos:inScheme base: .

<https://vocab.ifremer.fr/scheme/SXT/SNO/186247da-31da-48cf-8a97-9c3c7d6ed119> skos:broader <https://w3id.org/earthsemantics/ODATIS/SNO> ;
    skos:inScheme base: .

<https://vocab.ifremer.fr/scheme/SXT/SNO/2a7aa178-739e-4276-933b-1caa539d4aa6> skos:broader <https://w3id.org/earthsemantics/ODATIS/SNO> ;
    skos:inScheme base: .

<https://vocab.ifremer.fr/scheme/SXT/SNO/373eaec7-f331-47e4-8dd9-92bd1158dc13> skos:broader <https://w3id.org/earthsemantics/ODATIS/SNO> ;
    skos:inScheme base: .

<https://vocab.ifremer.fr/scheme/SXT/SNO/3ff86121-016b-4b2f-bad8-ea5825942032> skos:broader <https://w3id.org/earthsemantics/ODATIS/SNO> ;
    skos:inScheme base: .

<https://vocab.ifremer.fr/scheme/SXT/SNO/4ea9d6cf-4397-4e07-94e8-4393edfb4714> skos:broader <https://w3id.org/earthsemantics/ODATIS/SNO> ;
    skos:inScheme base: .

<https://vocab.ifremer.fr/scheme/SXT/SNO/50b221d3-9d8a-4987-8705-0c91fcaaa68f> skos:broader <https://w3id.org/earthsemantics/ODATIS/SNO> ;
    skos:inScheme base: .

<https://vocab.ifremer.fr/scheme/SXT/SNO/67ca6ff3-49b1-475c-a922-d80024810df8> skos:broader <https://w3id.org/earthsemantics/ODATIS/SNO> ;
    skos:inScheme base: .

<https://vocab.ifremer.fr/scheme/SXT/SNO/98b551e7-13e9-41d1-820a-34475b4b69a0> skos:broader <https://w3id.org/earthsemantics/ODATIS/SNO> ;
    skos:inScheme base: .

<https://vocab.ifremer.fr/scheme/SXT/SNO/9d775b58-3e42-4943-ad65-efcf210e4c6c> skos:broader <https://w3id.org/earthsemantics/ODATIS/SNO> ;
    skos:inScheme base: .

<https://vocab.ifremer.fr/scheme/SXT/SNO/a62b14be-c786-4aa1-bf45-f92a26d348bd> skos:broader <https://w3id.org/earthsemantics/ODATIS/SNO> ;
    skos:inScheme base: .

<https://vocab.ifremer.fr/scheme/SXT/SNO/aabea3b2-4ec1-4c09-bea5-21fd0e0b096f> skos:broader <https://w3id.org/earthsemantics/ODATIS/SNO> ;
    skos:inScheme base: .

<https://vocab.ifremer.fr/scheme/SXT/SNO/b32bf1b2-dab3-4b43-996c-6a4365e4159b> skos:broader <https://w3id.org/earthsemantics/ODATIS/SNO> ;
    skos:inScheme base: .

<https://vocab.ifremer.fr/scheme/SXT/SNO/b41e4ba1-3377-42d7-bbcc-9404b927ea3c> skos:broader <https://w3id.org/earthsemantics/ODATIS/SNO> ;
    skos:inScheme base: .

<https://vocab.ifremer.fr/scheme/SXT/SNO/b935ea2f-d349-4664-bf5a-f152f1d5c5bb> skos:broader <https://w3id.org/earthsemantics/ODATIS/SNO> ;
    skos:inScheme base: .

<https://vocab.ifremer.fr/scheme/SXT/SNO/ca4fb725-0f70-40a6-947f-33435b16c418> skos:broader <https://w3id.org/earthsemantics/ODATIS/SNO> ;
    skos:inScheme base: .

<https://vocab.ifremer.fr/scheme/SXT/SNO/e766ad56-824b-4d1e-9173-7a63aff65b70> skos:broader <https://w3id.org/earthsemantics/ODATIS/SNO> ;
    skos:inScheme base: .

<https://vocab.ifremer.fr/scheme/SXT/SNO/f2279789-e199-4617-90ce-1c8363085d28> skos:broader <https://w3id.org/earthsemantics/ODATIS/SNO> ;
    skos:inScheme base: .

<https://vocab.ifremer.fr/scheme/SXT/odatis_centre_donnees/1500646c-46f5-4da2-b6b2-2bfa6eb9415d> skos:broader <https://w3id.org/earthsemantics/ODATIS/odatis_centre_donnees> ;
    skos:inScheme base: .

<https://vocab.ifremer.fr/scheme/SXT/odatis_centre_donnees/34c66ea5-3b28-4a1f-9cd7-623c827dc525> skos:broader <https://w3id.org/earthsemantics/ODATIS/odatis_centre_donnees> ;
    skos:inScheme base: .

<https://vocab.ifremer.fr/scheme/SXT/odatis_centre_donnees/5c8a927b-6d39-4506-9b8b-88908a2974c3> skos:broader <https://w3id.org/earthsemantics/ODATIS/odatis_centre_donnees> ;
    skos:inScheme base: .

<https://vocab.ifremer.fr/scheme/SXT/odatis_centre_donnees/66b253d4-1e05-454b-9641-4e281c11431a> skos:broader <https://w3id.org/earthsemantics/ODATIS/odatis_centre_donnees> ;
    skos:inScheme base: .

<https://vocab.ifremer.fr/scheme/SXT/odatis_centre_donnees/720a0782-03c4-46a4-a35a-e5bd71d741b8> skos:broader <https://w3id.org/earthsemantics/ODATIS/odatis_centre_donnees> ;
    skos:inScheme base: .

<https://vocab.ifremer.fr/scheme/SXT/odatis_centre_donnees/730d8bf9-3a8c-4a21-bdf3-614968c5e3cb> skos:broader <https://w3id.org/earthsemantics/ODATIS/odatis_centre_donnees> ;
    skos:inScheme base: .

<https://vocab.ifremer.fr/scheme/SXT/odatis_centre_donnees/807b0273-8206-420f-91f4-e0dcdd13110c> skos:broader <https://w3id.org/earthsemantics/ODATIS/odatis_centre_donnees> ;
    skos:inScheme base: .

<https://vocab.ifremer.fr/scheme/SXT/odatis_centre_donnees/840271f5-c45f-46d3-9fcf-e23fcf802d71> skos:broader <https://w3id.org/earthsemantics/ODATIS/odatis_centre_donnees> ;
    skos:inScheme base: .

<https://vocab.ifremer.fr/scheme/SXT/odatis_centre_donnees/85787e11-f61e-4af7-a39a-bb9aea8d0447> skos:broader <https://w3id.org/earthsemantics/ODATIS/odatis_centre_donnees> ;
    skos:inScheme base: .

<https://vocab.ifremer.fr/scheme/SXT/type_jeux_donnee/308699d0-2a4a-40d3-a418-b0396dbe7534> skos:inScheme base: .

<https://vocab.ifremer.fr/scheme/SXT/type_jeux_donnee/5f6824e5-a2da-4f4c-a2cc-0a1aeb9d590c> skos:broader <https://w3id.org/earthsemantics/ODATIS/type_jeux_donnee> ;
    skos:inScheme base: .

<https://vocab.ifremer.fr/scheme/SXT/type_jeux_donnee/69c1d1e8-df22-458c-8daa-34c67bfb3f8d> skos:broader <https://w3id.org/earthsemantics/ODATIS/type_jeux_donnee> ;
    skos:inScheme base: .

<https://vocab.ifremer.fr/scheme/SXT/type_jeux_donnee/73360e4a-0082-4973-b1a1-836a728c8bbd> skos:broader <https://w3id.org/earthsemantics/ODATIS/type_jeux_donnee> ;
    skos:inScheme base: .

<https://vocab.ifremer.fr/scheme/SXT/type_jeux_donnee/ad1acbcb-a75a-4541-8214-c505c6c134bd> skos:broader <https://w3id.org/earthsemantics/ODATIS/type_jeux_donnee> ;
    skos:inScheme base: .

<https://vocab.ifremer.fr/scheme/SXT/type_jeux_donnee/c0d4cb33-61b7-4e83-8103-67c8b6a11671> skos:broader <https://w3id.org/earthsemantics/ODATIS/type_jeux_donnee> ;
    skos:inScheme base: .

<https://vocab.ifremer.fr/scheme/SXT/type_jeux_donnee/ee886158-f9cc-470d-b9cb-b2c7bec0fea2> skos:inScheme base: .

<http://vocab.nerc.ac.uk/collection/OD1/current/ACOUST/> a skos:Concept ;
    dc:identifier "SDN:OD1::ACOUST" ;
    dcterms:date "2023-09-28 13:57:47.0" ;
    dcterms:identifier "SDN:OD1::ACOUST" ;
    ns2:authoredOn "2023-09-28 13:57:47.0" ;
    ns2:hasCurrentVersion <http://vocab.nerc.ac.uk/collection/OD1/current/ACOUST/1/> ;
    ns2:version "1" ;
    void:inDataset <http://vocab.nerc.ac.uk/.well-known/void> ;
    owl:deprecated "false" ;
    owl:sameAs <http://vocab.nerc.ac.uk/collection/P03/current/D005/> ;
    owl:versionInfo "1" ;
    skos:altLabel "" ;
    skos:broader <http://vocab.nerc.ac.uk/collection/P08/current/DS03/> ;
    skos:definition "Scientific field of study pertaining to sound emission and propagation in the marine environment. This topic includes the measurement of sound characteristics and the information they provide in the fields of telluric and hydroclimatic risk, biodiversity inventory and evolution, and anthropic impact."@en,
        "Non displonible"@fr ;
    skos:notation "SDN:OD1::ACOUST" ;
    skos:note "accepted"@en ;
    skos:prefLabel "Ocean Acoustics"@en,
        "Acoustique de l'océan"@fr .

<http://vocab.nerc.ac.uk/collection/OD1/current/AERO/> a skos:Concept ;
    dc:identifier "SDN:OD1::AERO" ;
    dcterms:date "2023-09-28 13:57:47.0" ;
    dcterms:identifier "SDN:OD1::AERO" ;
    ns2:authoredOn "2023-09-28 13:57:47.0" ;
    ns2:hasCurrentVersion <http://vocab.nerc.ac.uk/collection/OD1/current/AERO/1/> ;
    ns2:version "1" ;
    void:inDataset <http://vocab.nerc.ac.uk/.well-known/void> ;
    owl:deprecated "false" ;
    owl:sameAs <http://vocab.nerc.ac.uk/collection/P02/current/ATPC/>,
        <https://gcmd.earthdata.nasa.gov/kms/concept/2e5a401b-1507-4f57-82b8-36557c13b154>,
        <https://gcos.wmo.int/en/essential-climate-variables/aerosols> ;
    owl:versionInfo "1" ;
    skos:altLabel "" ;
    skos:broader <http://vocab.nerc.ac.uk/collection/P03/current/M005/>,
        <http://vocab.nerc.ac.uk/collection/P08/current/DS05/> ;
    skos:definition "Suspension of particles of condensed matter (liquid, solid, or mixed) in a carrier gas (usually air). Aerosols are important in the atmosphere as nuclei for the condensation of water droplets and ice crystals, as participants in various chemical cycles, and as absorbers and scatterers of solar radiation, thereby influencing the radiation budget of the earth-atmosphere system, which in turn influences the climate on the surface of the Earth."@en,
        "Non displonible"@fr ;
    skos:notation "SDN:OD1::AERO" ;
    skos:note "accepted"@en ;
    skos:prefLabel "Aerosols"@en,
        "Aérosols"@fr .

<http://vocab.nerc.ac.uk/collection/OD1/current/AIRPRES/> a skos:Concept ;
    dc:identifier "SDN:OD1::AIRPRES" ;
    dcterms:date "2023-10-10 14:51:12.0" ;
    dcterms:identifier "SDN:OD1::AIRPRES" ;
    ns2:authoredOn "2023-10-10 14:51:12.0" ;
    ns2:hasCurrentVersion <http://vocab.nerc.ac.uk/collection/OD1/current/AIRPRES/1/> ;
    ns2:version "1" ;
    void:inDataset <http://vocab.nerc.ac.uk/.well-known/void> ;
    owl:deprecated "false" ;
    owl:sameAs <http://vocab.nerc.ac.uk/collection/A05/current/EV_AIRPRESS/>,
        <http://vocab.nerc.ac.uk/collection/P02/current/CAPH/>,
        <https://gcos.wmo.int/en/essential-climate-variables/pressure> ;
    owl:versionInfo "1" ;
    skos:altLabel "" ;
    skos:broader <http://vocab.nerc.ac.uk/collection/P03/current/M010/>,
        <http://vocab.nerc.ac.uk/collection/P08/current/DS05/> ;
    skos:definition "Variables associated with the determination of the atmospheric pressure near the Earth's surface."@en,
        "Non displonible"@fr ;
    skos:notation "SDN:OD1::AIRPRES" ;
    skos:note "accepted"@en ;
    skos:prefLabel "Atmospheric pressure"@en,
        "Pression atmosphérique"@fr .

<http://vocab.nerc.ac.uk/collection/OD1/current/AIRTEMP/> a skos:Concept ;
    dc:identifier "SDN:OD1::AIRTEMP" ;
    dcterms:date "2023-10-10 14:51:12.0" ;
    dcterms:identifier "SDN:OD1::AIRTEMP" ;
    ns2:authoredOn "2023-10-10 14:51:12.0" ;
    ns2:hasCurrentVersion <http://vocab.nerc.ac.uk/collection/OD1/current/AIRTEMP/1/> ;
    ns2:version "1" ;
    void:inDataset <http://vocab.nerc.ac.uk/.well-known/void> ;
    owl:deprecated "false" ;
    owl:sameAs <http://vocab.nerc.ac.uk/collection/A05/current/EV_AIRTEMP/>,
        <http://vocab.nerc.ac.uk/collection/P02/current/CDTA/>,
        <https://gcos.wmo.int/en/essential-climate-variables/surface-temperature> ;
    owl:versionInfo "1" ;
    skos:altLabel "" ;
    skos:broader <http://vocab.nerc.ac.uk/collection/P03/current/M010/>,
        <http://vocab.nerc.ac.uk/collection/P08/current/DS05/> ;
    skos:definition "Variables associated with the determination of the air temperature near the Earth's surface."@en,
        "Non displonible"@fr ;
    skos:notation "SDN:OD1::AIRTEMP" ;
    skos:note "accepted"@en ;
    skos:prefLabel "Air temperature"@en,
        "Température de l'air"@fr .

<http://vocab.nerc.ac.uk/collection/OD1/current/BATHY/> a skos:Concept ;
    dc:identifier "SDN:OD1::BATHY" ;
    dcterms:date "2023-09-28 13:57:47.0" ;
    dcterms:identifier "SDN:OD1::BATHY" ;
    ns2:authoredOn "2023-09-28 13:57:47.0" ;
    ns2:hasCurrentVersion <http://vocab.nerc.ac.uk/collection/OD1/current/BATHY/1/> ;
    ns2:version "1" ;
    void:inDataset <http://vocab.nerc.ac.uk/.well-known/void> ;
    owl:deprecated "false" ;
    owl:sameAs <http://vocab.nerc.ac.uk/collection/P03/current/G005/> ;
    owl:versionInfo "1" ;
    skos:altLabel "" ;
    skos:broader <http://vocab.nerc.ac.uk/collection/P02/current/MBAN/>,
        <http://vocab.nerc.ac.uk/collection/P08/current/DS04/> ;
    skos:definition "Science and technology of measuring or estimating depth. Its aim is to determine the relief of the deep or coastal ocean."@en,
        "Non displonible"@fr ;
    skos:narrower <http://vocab.nerc.ac.uk/collection/A05/current/EV_BATHY/> ;
    skos:notation "SDN:OD1::BATHY" ;
    skos:note "accepted"@en ;
    skos:prefLabel "Bathymetry"@en,
        "Bathymétrie"@fr .

<http://vocab.nerc.ac.uk/collection/OD1/current/BENTHA/> a skos:Concept ;
    dc:identifier "SDN:OD1::BENTHA" ;
    dcterms:date "2023-09-28 13:57:47.0" ;
    dcterms:identifier "SDN:OD1::BENTHA" ;
    ns2:authoredOn "2023-09-28 13:57:47.0" ;
    ns2:hasCurrentVersion <http://vocab.nerc.ac.uk/collection/OD1/current/BENTHA/1/> ;
    ns2:version "1" ;
    void:inDataset <http://vocab.nerc.ac.uk/.well-known/void> ;
    owl:deprecated "false" ;
    owl:sameAs <http://vocab.nerc.ac.uk/collection/P03/current/B050/>,
        <https://gcos.wmo.int/en/essential-climate-variables/marine-habitats/> ;
    owl:versionInfo "1" ;
    skos:altLabel "" ;
    skos:broader <http://vocab.nerc.ac.uk/collection/P02/current/HBCH/>,
        <http://vocab.nerc.ac.uk/collection/P02/current/HBEX/>,
        <http://vocab.nerc.ac.uk/collection/P08/current/DS10/> ;
    skos:definition "Marine benthic habitats are the bed of seas directly connected to the oceans, i.e. part of the continuous body of water which covers the greater part of the earth."@en,
        "Non displonible"@fr ;
    skos:notation "SDN:OD1::BENTHA" ;
    skos:note "accepted"@en ;
    skos:prefLabel "Benthic habitats"@en,
        "Habitats benthiques"@fr .

<http://vocab.nerc.ac.uk/collection/OD1/current/BIOINFO/> a skos:Concept ;
    dc:identifier "SDN:OD1::BIOINFO" ;
    dcterms:date "2023-09-28 13:57:47.0" ;
    dcterms:identifier "SDN:OD1::BIOINFO" ;
    ns2:authoredOn "2023-09-28 13:57:47.0" ;
    ns2:hasCurrentVersion <http://vocab.nerc.ac.uk/collection/OD1/current/BIOINFO/1/> ;
    ns2:version "1" ;
    void:inDataset <http://vocab.nerc.ac.uk/.well-known/void> ;
    owl:deprecated "false" ;
    owl:versionInfo "1" ;
    skos:altLabel "" ;
    skos:broader <http://vocab.nerc.ac.uk/collection/P03/current/B070/>,
        <http://vocab.nerc.ac.uk/collection/P03/current/C050/>,
        <http://vocab.nerc.ac.uk/collection/P08/current/DS01/>,
        <http://vocab.nerc.ac.uk/collection/P08/current/DS02/> ;
    skos:definition "Interdisciplinary field of science that develops methods and software tools for understanding biological data, especially when the data sets are large and complex."@en,
        "Non displonible"@fr ;
    skos:notation "SDN:OD1::BIOINFO" ;
    skos:note "accepted"@en ;
    skos:prefLabel "Bioinformatics"@en,
        "Bioinformatique"@fr .

<http://vocab.nerc.ac.uk/collection/OD1/current/BIOTOX/> a skos:Concept ;
    dc:identifier "SDN:OD1::BIOTOX" ;
    dcterms:date "2023-10-10 14:51:12.0" ;
    dcterms:identifier "SDN:OD1::BIOTOX" ;
    ns2:authoredOn "2023-10-10 14:51:12.0" ;
    ns2:hasCurrentVersion <http://vocab.nerc.ac.uk/collection/OD1/current/BIOTOX/1/> ;
    ns2:version "1" ;
    void:inDataset <http://vocab.nerc.ac.uk/.well-known/void> ;
    owl:deprecated "false" ;
    owl:sameAs <http://vocab.nerc.ac.uk/collection/P02/current/BCOC/>,
        <http://vocab.nerc.ac.uk/collection/P02/current/PTOX/> ;
    owl:versionInfo "1" ;
    skos:altLabel "" ;
    skos:broader <http://vocab.nerc.ac.uk/collection/P03/current/B007/>,
        <http://vocab.nerc.ac.uk/collection/P03/current/C055/>,
        <http://vocab.nerc.ac.uk/collection/P03/current/H001/>,
        <http://vocab.nerc.ac.uk/collection/P08/current/DS02/> ;
    skos:definition "Toxins are contaminants secreted by certain algae or phytoplankton; they are called phycotoxins or marine biotoxins."@en,
        "Non displonible"@fr ;
    skos:notation "SDN:OD1::BIOTOX" ;
    skos:note "accepted"@en ;
    skos:prefLabel "Biotoxins"@en,
        "Biotoxines"@fr .

<http://vocab.nerc.ac.uk/collection/OD1/current/C02/> a skos:Concept ;
    dc:identifier "SDN:OD1::C02" ;
    dcterms:date "2023-09-28 13:57:47.0" ;
    dcterms:identifier "SDN:OD1::C02" ;
    ns2:authoredOn "2023-09-28 13:57:47.0" ;
    ns2:hasCurrentVersion <http://vocab.nerc.ac.uk/collection/OD1/current/C02/1/> ;
    ns2:version "1" ;
    void:inDataset <http://vocab.nerc.ac.uk/.well-known/void> ;
    owl:deprecated "false" ;
    owl:sameAs <http://vocab.nerc.ac.uk/collection/A05/current/EV_CO2/>,
        <http://vocab.nerc.ac.uk/collection/P03/current/C010/> ;
    owl:versionInfo "1" ;
    skos:altLabel "" ;
    skos:broader <http://vocab.nerc.ac.uk/collection/P02/current/ALKY/>,
        <http://vocab.nerc.ac.uk/collection/P02/current/CCPW/>,
        <http://vocab.nerc.ac.uk/collection/P02/current/PCO2/>,
        <http://vocab.nerc.ac.uk/collection/P02/current/PHLT/>,
        <http://vocab.nerc.ac.uk/collection/P02/current/TCO2/>,
        <http://vocab.nerc.ac.uk/collection/P08/current/DS02/> ;
    skos:definition "The chemistry of carbon dioxide (DIC, TA, pCO2 and pH) in seawater where pH is expressed against Total, Seawater or Free scales. Includes water column and atmospheric measurements."@en,
        "Non displonible"@fr ;
    skos:notation "SDN:OD1::C02" ;
    skos:note "accepted"@en ;
    skos:prefLabel "CO2 Carbonate system"@en,
        "CO2 Système de carbonate"@fr .

<http://vocab.nerc.ac.uk/collection/OD1/current/COLOUR/> a skos:Concept ;
    dc:identifier "SDN:OD1::COLOUR" ;
    dcterms:date "2023-09-28 13:57:47.0" ;
    dcterms:identifier "SDN:OD1::COLOUR" ;
    ns2:authoredOn "2023-09-28 13:57:47.0" ;
    ns2:hasCurrentVersion <http://vocab.nerc.ac.uk/collection/OD1/current/COLOUR/1/> ;
    ns2:version "1" ;
    void:inDataset <http://vocab.nerc.ac.uk/.well-known/void> ;
    owl:deprecated "false" ;
    owl:versionInfo "1" ;
    skos:altLabel "" ;
    skos:broader <http://vocab.nerc.ac.uk/collection/P02/current/R410/>,
        <http://vocab.nerc.ac.uk/collection/P03/current/D015/>,
        <http://vocab.nerc.ac.uk/collection/P08/current/DS03/> ;
    skos:definition "Spectral radiance emanating from the sun that is backscattered off the upper part of the oceanic water column, and which contains information on the properties of the water and its constituents."@en,
        "Non displonible"@fr ;
    skos:notation "SDN:OD1::COLOUR" ;
    skos:note "accepted"@en ;
    skos:prefLabel "Ocean colour"@en,
        "Couleur de l'océan"@fr .

<http://vocab.nerc.ac.uk/collection/OD1/current/CONT/> a skos:Concept ;
    dc:identifier "SDN:OD1::CONT" ;
    dcterms:date "2023-09-28 13:57:47.0" ;
    dcterms:identifier "SDN:OD1::CONT" ;
    ns2:authoredOn "2023-09-28 13:57:47.0" ;
    ns2:hasCurrentVersion <http://vocab.nerc.ac.uk/collection/OD1/current/CONT/1/> ;
    ns2:version "1" ;
    void:inDataset <http://vocab.nerc.ac.uk/.well-known/void> ;
    owl:deprecated "false" ;
    owl:versionInfo "1" ;
    skos:altLabel "" ;
    skos:broader <http://vocab.nerc.ac.uk/collection/P02/current/BCAH/>,
        <http://vocab.nerc.ac.uk/collection/P02/current/BCMT/>,
        <http://vocab.nerc.ac.uk/collection/P02/current/BCPB/>,
        <http://vocab.nerc.ac.uk/collection/P02/current/BLIT/>,
        <http://vocab.nerc.ac.uk/collection/P02/current/MDBO/>,
        <http://vocab.nerc.ac.uk/collection/P02/current/PEBI/>,
        <http://vocab.nerc.ac.uk/collection/P03/current/C025/>,
        <http://vocab.nerc.ac.uk/collection/P03/current/C035/>,
        <http://vocab.nerc.ac.uk/collection/P03/current/C055/>,
        <http://vocab.nerc.ac.uk/collection/P03/current/H001/>,
        <http://vocab.nerc.ac.uk/collection/P08/current/DS02/>,
        <http://vocab.nerc.ac.uk/collection/P08/current/DS10/>,
        <http://vocab.nerc.ac.uk/collection/P08/current/DS12/> ;
    skos:definition "Pollutants coming from human activities on land and in the sea, including antifoulants (Organometallic spicies concentration); Hydrocarbons (Concentration of polycyclic aromatic hydrocarbons); Polychlorinated biphenyls (Concentration of polychlorobiphenyls); Pesticides and biocides (Pesticide concentrations); Heavy metals (Metal concentrations, Inorganic chemical composition)."@en,
        "Non displonible"@fr ;
    skos:notation "SDN:OD1::CONT" ;
    skos:note "accepted"@en ;
    skos:prefLabel "Contaminants"@en,
        "Contaminants"@fr .

<http://vocab.nerc.ac.uk/collection/OD1/current/CURR/> a skos:Concept ;
    dc:identifier "SDN:OD1::CURR" ;
    dcterms:date "2023-10-10 14:51:12.0" ;
    dcterms:identifier "SDN:OD1::CURR" ;
    ns2:authoredOn "2023-10-10 14:51:12.0" ;
    ns2:hasCurrentVersion <http://vocab.nerc.ac.uk/collection/OD1/current/CURR/1/> ;
    ns2:version "1" ;
    void:inDataset <http://vocab.nerc.ac.uk/.well-known/void> ;
    owl:deprecated "false" ;
    owl:sameAs <http://vocab.nerc.ac.uk/collection/A05/current/EV_CURR/>,
        <http://vocab.nerc.ac.uk/collection/P03/current/D030/> ;
    owl:versionInfo "1" ;
    skos:altLabel "" ;
    skos:broader <http://vocab.nerc.ac.uk/collection/P08/current/DS03/> ;
    skos:definition "Variables associated with the determination of the speed and direction of surface and subsuface seawater currents."@en,
        "Non displonible"@fr ;
    skos:narrower <https://gcos.wmo.int/en/essential-climate-variables/subsurface-currents>,
        <https://gcos.wmo.int/en/essential-climate-variables/surface-currents> ;
    skos:notation "SDN:OD1::CURR" ;
    skos:note "accepted"@en ;
    skos:prefLabel "Currents"@en,
        "Courants"@fr .

<http://vocab.nerc.ac.uk/collection/OD1/current/DENS/> a skos:Concept ;
    dc:identifier "SDN:OD1::DENS" ;
    dcterms:date "2024-06-06 16:49:45.0" ;
    dcterms:identifier "SDN:OD1::DENS" ;
    ns2:authoredOn "2024-06-06 16:49:45.0" ;
    ns2:hasCurrentVersion <http://vocab.nerc.ac.uk/collection/OD1/current/DENS/1/> ;
    ns2:version "1" ;
    void:inDataset <http://vocab.nerc.ac.uk/.well-known/void> ;
    owl:deprecated "false" ;
    owl:sameAs <http://vocab.nerc.ac.uk/collection/P02/current/CAPH/>,
        <http://vocab.nerc.ac.uk/collection/P02/current/DBDX/>,
        <http://vocab.nerc.ac.uk/collection/P02/current/SIGT/> ;
    owl:versionInfo "1" ;
    skos:altLabel "" ;
    skos:broader <http://vocab.nerc.ac.uk/collection/P03/current/M010/>,
        <http://vocab.nerc.ac.uk/collection/P08/current/DS05/> ;
    skos:definition "The mass per unit volume of a substance."@en,
        "Non displonible"@fr ;
    skos:notation "SDN:OD1::DENS" ;
    skos:note "accepted"@en ;
    skos:prefLabel "Density"@en,
        "Densité"@fr .

<http://vocab.nerc.ac.uk/collection/OD1/current/DOM/> a skos:Concept ;
    dc:identifier "SDN:OD1::DOM" ;
    dcterms:date "2023-09-28 13:57:47.0" ;
    dcterms:identifier "SDN:OD1::DOM" ;
    ns2:authoredOn "2023-09-28 13:57:47.0" ;
    ns2:hasCurrentVersion <http://vocab.nerc.ac.uk/collection/OD1/current/DOM/1/> ;
    ns2:version "1" ;
    void:inDataset <http://vocab.nerc.ac.uk/.well-known/void> ;
    owl:deprecated "false" ;
    owl:sameAs <http://vocab.nerc.ac.uk/collection/A05/current/EV_DOM/> ;
    owl:versionInfo "1" ;
    skos:altLabel "" ;
    skos:broader <http://vocab.nerc.ac.uk/collection/P02/current/DOCC/>,
        <http://vocab.nerc.ac.uk/collection/P02/current/TDIN/>,
        <http://vocab.nerc.ac.uk/collection/P02/current/TDNT/>,
        <http://vocab.nerc.ac.uk/collection/P02/current/TDPX/>,
        <http://vocab.nerc.ac.uk/collection/P03/current/C005/>,
        <http://vocab.nerc.ac.uk/collection/P08/current/DS02/> ;
    skos:definition "The amount of dissolved organic matter (DOC, DON and CDOM) in seawater using water column measurements."@en,
        "Non displonible"@fr ;
    skos:notation "SDN:OD1::DOM" ;
    skos:note "accepted"@en ;
    skos:prefLabel "Dissolved Organic Matter"@en,
        "Matière organique dissoute"@fr .

<http://vocab.nerc.ac.uk/collection/OD1/current/DOXY/> a skos:Concept ;
    dc:identifier "SDN:OD1::DOXY" ;
    dcterms:date "2023-10-10 14:51:12.0" ;
    dcterms:identifier "SDN:OD1::DOXY" ;
    ns2:authoredOn "2023-10-10 14:51:12.0" ;
    ns2:hasCurrentVersion <http://vocab.nerc.ac.uk/collection/OD1/current/DOXY/1/> ;
    ns2:version "1" ;
    void:inDataset <http://vocab.nerc.ac.uk/.well-known/void> ;
    owl:deprecated "false" ;
    owl:sameAs <http://vocab.nerc.ac.uk/collection/A05/current/EV_OXY/>,
        <http://vocab.nerc.ac.uk/collection/P02/current/DOXY/> ;
    owl:versionInfo "1" ;
    skos:altLabel "" ;
    skos:broader <http://vocab.nerc.ac.uk/collection/P03/current/C015/>,
        <http://vocab.nerc.ac.uk/collection/P08/current/DS02/> ;
    skos:definition "Variables associated with the determination of the amount of oxygen dissolved in seawater using water column measurements."@en,
        "Non displonible"@fr ;
    skos:notation "SDN:OD1::DOXY" ;
    skos:note "accepted"@en ;
    skos:prefLabel "Dissolved oxygen"@en,
        "Oxygène dissous"@fr .

<http://vocab.nerc.ac.uk/collection/OD1/current/FISH/> a skos:Concept ;
    dc:identifier "SDN:OD1::FISH" ;
    dcterms:date "2024-06-06 16:49:45.0" ;
    dcterms:identifier "SDN:OD1::FISH" ;
    ns2:authoredOn "2024-06-06 16:49:45.0" ;
    ns2:hasCurrentVersion <http://vocab.nerc.ac.uk/collection/OD1/current/FISH/1/> ;
    ns2:version "1" ;
    void:inDataset <http://vocab.nerc.ac.uk/.well-known/void> ;
    owl:deprecated "false" ;
    owl:sameAs <http://vocab.nerc.ac.uk/collection/P03/current/B020/> ;
    owl:versionInfo "1" ;
    skos:altLabel "" ;
    skos:broader <http://vocab.nerc.ac.uk/collection/P08/current/DS01/>,
        <http://vocab.nerc.ac.uk/collection/P08/current/DS11/> ;
    skos:definition "This group incorporates all state variables pertaining to fish, such as abundance, biomass and fisheries data."@en,
        "Non displonible"@fr ;
    skos:notation "SDN:OD1::FISH" ;
    skos:note "accepted"@en ;
    skos:prefLabel "Fish"@en,
        "Poissons"@fr .

<http://vocab.nerc.ac.uk/collection/OD1/current/FLUO/> a skos:Concept ;
    dc:identifier "SDN:OD1::FLUO" ;
    dcterms:date "2024-06-06 16:49:45.0" ;
    dcterms:identifier "SDN:OD1::FLUO" ;
    ns2:authoredOn "2024-06-06 16:49:45.0" ;
    ns2:hasCurrentVersion <http://vocab.nerc.ac.uk/collection/OD1/current/FLUO/1/> ;
    ns2:version "1" ;
    void:inDataset <http://vocab.nerc.ac.uk/.well-known/void> ;
    owl:deprecated "false" ;
    owl:sameAs <http://vocab.nerc.ac.uk/collection/P02/current/CMFL/>,
        <http://vocab.nerc.ac.uk/collection/P02/current/FVLT/> ;
    owl:versionInfo "1" ;
    skos:altLabel "" ;
    skos:broader <http://vocab.nerc.ac.uk/collection/P03/current/O010/>,
        <http://vocab.nerc.ac.uk/collection/P08/current/DS06/> ;
    skos:definition "The emission of radiation, especially of visible light, by a substance during exposure to external radiation, as light or x-rays."@en,
        "Non displonible"@fr ;
    skos:notation "SDN:OD1::FLUO" ;
    skos:note "accepted"@en ;
    skos:prefLabel "Fluorescence"@en,
        "Fluorescence"@fr .

<http://vocab.nerc.ac.uk/collection/OD1/current/GEOL/> a skos:Concept ;
    dc:identifier "SDN:OD1::GEOL" ;
    dcterms:date "2024-06-06 16:49:45.0" ;
    dcterms:identifier "SDN:OD1::GEOL" ;
    ns2:authoredOn "2024-06-06 16:49:45.0" ;
    ns2:hasCurrentVersion <http://vocab.nerc.ac.uk/collection/OD1/current/GEOL/1/> ;
    ns2:version "1" ;
    void:inDataset <http://vocab.nerc.ac.uk/.well-known/void> ;
    owl:deprecated "false" ;
    owl:sameAs <http://vocab.nerc.ac.uk/collection/P08/current/DS04/> ;
    owl:versionInfo "1" ;
    skos:altLabel "" ;
    skos:definition "The marine geological science domain."@en,
        "Non displonible"@fr ;
    skos:notation "SDN:OD1::GEOL" ;
    skos:note "accepted"@en ;
    skos:prefLabel "Geology"@en,
        "Géologie"@fr .

<http://vocab.nerc.ac.uk/collection/OD1/current/HCORAL/> a skos:Concept ;
    dc:identifier "SDN:OD1::HCORAL" ;
    dcterms:date "2024-06-06 16:49:45.0" ;
    dcterms:identifier "SDN:OD1::HCORAL" ;
    ns2:authoredOn "2024-06-06 16:49:45.0" ;
    ns2:hasCurrentVersion <http://vocab.nerc.ac.uk/collection/OD1/current/HCORAL/1/> ;
    ns2:version "1" ;
    void:inDataset <http://vocab.nerc.ac.uk/.well-known/void> ;
    owl:deprecated "false" ;
    owl:versionInfo "1" ;
    skos:altLabel "" ;
    skos:definition "Cover and composition of hard coral."@en,
        "Non displonible"@fr ;
    skos:notation "SDN:OD1::HCORAL" ;
    skos:note "accepted"@en ;
    skos:prefLabel "Hard coral"@en,
        "Coraux"@fr .

<http://vocab.nerc.ac.uk/collection/OD1/current/HEATCON/> a skos:Concept ;
    dc:identifier "SDN:OD1::HEATCON" ;
    dcterms:date "2023-09-28 13:57:47.0" ;
    dcterms:identifier "SDN:OD1::HEATCON" ;
    ns2:authoredOn "2023-09-28 13:57:47.0" ;
    ns2:hasCurrentVersion <http://vocab.nerc.ac.uk/collection/OD1/current/HEATCON/1/> ;
    ns2:version "1" ;
    void:inDataset <http://vocab.nerc.ac.uk/.well-known/void> ;
    owl:deprecated "false" ;
    owl:versionInfo "1" ;
    skos:altLabel "" ;
    skos:broader <http://vocab.nerc.ac.uk/collection/P08/current/DS03/> ;
    skos:definition "Study of the ocean content change from which the Earth Energy Imbalance can be inferred. Variables include the terms in the sea level budget equation. Different types of calculation based on absolute budgets or trends."@en,
        "Non displonible"@fr ;
    skos:notation "SDN:OD1::HEATCON" ;
    skos:note "accepted"@en ;
    skos:prefLabel "Ocean heat content"@en,
        "Contenu thermique de l'océan"@fr .

<http://vocab.nerc.ac.uk/collection/OD1/current/HUMACT/> a skos:Concept ;
    dc:identifier "SDN:OD1::HUMACT" ;
    dcterms:date "2024-06-06 16:49:45.0" ;
    dcterms:identifier "SDN:OD1::HUMACT" ;
    ns2:authoredOn "2024-06-06 16:49:45.0" ;
    ns2:hasCurrentVersion <http://vocab.nerc.ac.uk/collection/OD1/current/HUMACT/1/> ;
    ns2:version "1" ;
    void:inDataset <http://vocab.nerc.ac.uk/.well-known/void> ;
    owl:deprecated "false" ;
    owl:sameAs <http://vocab.nerc.ac.uk/collection/P08/current/DS12/> ;
    owl:versionInfo "1" ;
    skos:altLabel "" ;
    skos:definition "The domain documenting the activities of man that have an effect on the Earth System."@en,
        "Non displonible"@fr ;
    skos:notation "SDN:OD1::HUMACT" ;
    skos:note "accepted"@en ;
    skos:prefLabel "Human activities"@en,
        "Activités humaines"@fr .

<http://vocab.nerc.ac.uk/collection/OD1/current/HUMI/> a skos:Concept ;
    dc:identifier "SDN:OD1::HUMI" ;
    dcterms:date "2023-10-16 17:23:15.0" ;
    dcterms:identifier "SDN:OD1::HUMI" ;
    ns2:authoredOn "2023-10-16 17:23:15.0" ;
    ns2:hasCurrentVersion <http://vocab.nerc.ac.uk/collection/OD1/current/HUMI/1/> ;
    ns2:version "1" ;
    void:inDataset <http://vocab.nerc.ac.uk/.well-known/void> ;
    owl:deprecated "false" ;
    owl:sameAs <http://vocab.nerc.ac.uk/collection/A05/current/EV_AIRHUM/>,
        <http://vocab.nerc.ac.uk/collection/P02/current/CHUM/> ;
    owl:versionInfo "1" ;
    skos:altLabel "" ;
    skos:broader <http://vocab.nerc.ac.uk/collection/P03/current/M010/>,
        <http://vocab.nerc.ac.uk/collection/P08/current/DS05/> ;
    skos:definition "The amount of water vapour (relative humidity, dew point temperature) in the atmosphere."@en,
        "Non displonible"@fr ;
    skos:narrower <https://gcos.wmo.int/en/essential-climate-variables/surface-vapour> ;
    skos:notation "SDN:OD1::HUMI" ;
    skos:note "accepted"@en ;
    skos:prefLabel "Humidity"@en,
        "Humidité"@fr .

<http://vocab.nerc.ac.uk/collection/OD1/current/INVER/> a skos:Concept ;
    dc:identifier "SDN:OD1::INVER" ;
    dcterms:date "2023-09-28 13:57:47.0" ;
    dcterms:identifier "SDN:OD1::INVER" ;
    ns2:authoredOn "2023-09-28 13:57:47.0" ;
    ns2:hasCurrentVersion <http://vocab.nerc.ac.uk/collection/OD1/current/INVER/1/> ;
    ns2:version "1" ;
    void:inDataset <http://vocab.nerc.ac.uk/.well-known/void> ;
    owl:deprecated "false" ;
    owl:versionInfo "1" ;
    skos:altLabel "" ;
    skos:broader <http://vocab.nerc.ac.uk/collection/P03/current/B070/>,
        <http://vocab.nerc.ac.uk/collection/P08/current/DS01/> ;
    skos:definition "An animal lacking a vertebral column."@en,
        "Non displonible"@fr ;
    skos:notation "SDN:OD1::INVER" ;
    skos:note "accepted"@en ;
    skos:prefLabel "Invertebrates"@en,
        "Invertébrés"@fr .

<http://vocab.nerc.ac.uk/collection/OD1/current/MACALG/> a skos:Concept ;
    dc:identifier "SDN:OD1::MACALG" ;
    dcterms:date "2024-06-06 16:49:45.0" ;
    dcterms:identifier "SDN:OD1::MACALG" ;
    ns2:authoredOn "2024-06-06 16:49:45.0" ;
    ns2:hasCurrentVersion <http://vocab.nerc.ac.uk/collection/OD1/current/MACALG/1/> ;
    ns2:version "1" ;
    void:inDataset <http://vocab.nerc.ac.uk/.well-known/void> ;
    owl:deprecated "false" ;
    owl:sameAs <http://vocab.nerc.ac.uk/collection/P03/current/B055/> ;
    owl:versionInfo "1" ;
    skos:altLabel "" ;
    skos:broader <http://vocab.nerc.ac.uk/collection/P08/current/DS01/> ;
    skos:definition "Parameters pertaining to macroalgal."@en,
        "Non displonible"@fr ;
    skos:notation "SDN:OD1::MACALG" ;
    skos:note "accepted"@en ;
    skos:prefLabel "Macroalgal"@en,
        "Macroalgues"@fr .

<http://vocab.nerc.ac.uk/collection/OD1/current/MANG/> a skos:Concept ;
    dc:identifier "SDN:OD1::MANG" ;
    dcterms:date "2024-06-06 16:49:45.0" ;
    dcterms:identifier "SDN:OD1::MANG" ;
    ns2:authoredOn "2024-06-06 16:49:45.0" ;
    ns2:hasCurrentVersion <http://vocab.nerc.ac.uk/collection/OD1/current/MANG/1/> ;
    ns2:version "1" ;
    void:inDataset <http://vocab.nerc.ac.uk/.well-known/void> ;
    owl:deprecated "false" ;
    owl:versionInfo "1" ;
    skos:altLabel "" ;
    skos:broader <http://vocab.nerc.ac.uk/collection/P03/current/B050/>,
        <http://vocab.nerc.ac.uk/collection/P08/current/DS10/> ;
    skos:definition "Cover and composition of mangrove."@en,
        "Non displonible"@fr ;
    skos:notation "SDN:OD1::MANG" ;
    skos:note "accepted"@en ;
    skos:prefLabel "Mangrove"@en,
        "Mangroves"@fr .

<http://vocab.nerc.ac.uk/collection/OD1/current/MTBM/> a skos:Concept ;
    dc:identifier "SDN:OD1::MTBM" ;
    dcterms:date "2024-06-06 16:49:45.0" ;
    dcterms:identifier "SDN:OD1::MTBM" ;
    ns2:authoredOn "2024-06-06 16:49:45.0" ;
    ns2:hasCurrentVersion <http://vocab.nerc.ac.uk/collection/OD1/current/MTBM/1/> ;
    ns2:version "1" ;
    void:inDataset <http://vocab.nerc.ac.uk/.well-known/void> ;
    owl:deprecated "false" ;
    owl:sameAs <http://vocab.nerc.ac.uk/collection/P03/current/B015/> ;
    owl:versionInfo "1" ;
    skos:altLabel "" ;
    skos:broader <http://vocab.nerc.ac.uk/collection/P08/current/DS01/> ;
    skos:definition "This group incorporates all variables pertaining to marine turtles, birds,and mammals, including abundance, biomass, biological function and state of health."@en,
        "Non displonible"@fr ;
    skos:notation "SDN:OD1::MTBM" ;
    skos:note "accepted"@en ;
    skos:prefLabel "Marine turtles, birds, mammals"@en,
        "Tortues de mer, oiseaux et mammifères"@fr .

<http://vocab.nerc.ac.uk/collection/OD1/current/N2O/> a skos:Concept ;
    dc:identifier "SDN:OD1::N2O" ;
    dcterms:date "2023-10-10 14:51:12.0" ;
    dcterms:identifier "SDN:OD1::N2O" ;
    ns2:authoredOn "2023-10-10 14:51:12.0" ;
    ns2:hasCurrentVersion <http://vocab.nerc.ac.uk/collection/OD1/current/N2O/1/> ;
    ns2:version "1" ;
    void:inDataset <http://vocab.nerc.ac.uk/.well-known/void> ;
    owl:deprecated "false" ;
    owl:sameAs <http://vocab.nerc.ac.uk/collection/A05/current/EV_N2O/>,
        <https://gcos.wmo.int/en/essential-climate-variables/n2o/> ;
    owl:versionInfo "1" ;
    skos:altLabel "" ;
    skos:broader <http://vocab.nerc.ac.uk/collection/P02/current/SCOX/>,
        <http://vocab.nerc.ac.uk/collection/P03/current/C015/>,
        <http://vocab.nerc.ac.uk/collection/P08/current/DS02/> ;
    skos:definition "Variables associated with the determination of the amount of nitrous oxide in seawater using water column and atmospheric measurements."@en,
        "Non displonible"@fr ;
    skos:notation "SDN:OD1::N2O" ;
    skos:note "accepted"@en ;
    skos:prefLabel "Nitrous oxide"@en,
        "Oxyde d'azote"@fr .

<http://vocab.nerc.ac.uk/collection/OD1/current/NUTS/> a skos:Concept ;
    dc:identifier "SDN:OD1::NUTS" ;
    dcterms:date "2023-10-10 14:51:12.0" ;
    dcterms:identifier "SDN:OD1::NUTS" ;
    ns2:authoredOn "2023-10-10 14:51:12.0" ;
    ns2:hasCurrentVersion <http://vocab.nerc.ac.uk/collection/OD1/current/NUTS/1/> ;
    ns2:version "1" ;
    void:inDataset <http://vocab.nerc.ac.uk/.well-known/void> ;
    owl:deprecated "false" ;
    owl:sameAs <http://vocab.nerc.ac.uk/collection/A05/current/EV_NUTS/>,
        <http://vocab.nerc.ac.uk/collection/P03/current/C040/> ;
    owl:versionInfo "1" ;
    skos:altLabel "" ;
    skos:broader <http://vocab.nerc.ac.uk/collection/P08/current/DS02/> ;
    skos:definition "Variables associated with the determination of the amount of dissolved inorganic macronutrients (nitrate (NO3), phosphate (PO4), silicic acid (Si(OH)4), ammonium (NH4), nitrite (NO2)) in seawater using water column measurements."@en,
        "Non displonible"@fr ;
    skos:notation "SDN:OD1::NUTS" ;
    skos:note "accepted"@en ;
    skos:prefLabel "Nutrients"@en,
        "Nutriments"@fr .

<http://vocab.nerc.ac.uk/collection/OD1/current/PATHOGEN/> a skos:Concept ;
    dc:identifier "SDN:OD1::PATHOGEN" ;
    dcterms:date "2023-09-28 13:57:47.0" ;
    dcterms:identifier "SDN:OD1::PATHOGEN" ;
    ns2:authoredOn "2023-09-28 13:57:47.0" ;
    ns2:hasCurrentVersion <http://vocab.nerc.ac.uk/collection/OD1/current/PATHOGEN/1/> ;
    ns2:version "1" ;
    void:inDataset <http://vocab.nerc.ac.uk/.well-known/void> ;
    owl:deprecated "false" ;
    owl:sameAs <http://vocab.nerc.ac.uk/collection/P03/current/B005/> ;
    owl:versionInfo "1" ;
    skos:altLabel "" ;
    skos:broader <http://vocab.nerc.ac.uk/collection/P03/current/B060/>,
        <http://vocab.nerc.ac.uk/collection/P08/current/DS01/> ;
    skos:definition "Infectious agents (viruses, bacteria, parasites) considered as harmful, that could interact with the evolution of farming performances or cause enzootic disease."@en,
        "Non displonible"@fr ;
    skos:notation "SDN:OD1::PATHOGEN" ;
    skos:note "accepted"@en ;
    skos:prefLabel "Pathogenic organisms"@en,
        "Organismes pathogènes"@fr .

<http://vocab.nerc.ac.uk/collection/OD1/current/PHYTO/> a skos:Concept ;
    dc:identifier "SDN:OD1::PHYTO" ;
    dcterms:date "2023-09-28 13:57:47.0" ;
    dcterms:identifier "SDN:OD1::PHYTO" ;
    ns2:authoredOn "2023-09-28 13:57:47.0" ;
    ns2:hasCurrentVersion <http://vocab.nerc.ac.uk/collection/OD1/current/PHYTO/1/> ;
    ns2:version "1" ;
    void:inDataset <http://vocab.nerc.ac.uk/.well-known/void> ;
    owl:deprecated "false" ;
    owl:versionInfo "1" ;
    skos:altLabel "" ;
    skos:broader <http://vocab.nerc.ac.uk/collection/P02/current/CATX/>,
        <http://vocab.nerc.ac.uk/collection/P02/current/CNTX/>,
        <http://vocab.nerc.ac.uk/collection/P02/current/PATX/>,
        <http://vocab.nerc.ac.uk/collection/P02/current/PNTX/>,
        <http://vocab.nerc.ac.uk/collection/P02/current/VATX/>,
        <http://vocab.nerc.ac.uk/collection/P03/current/B030/>,
        <http://vocab.nerc.ac.uk/collection/P08/current/DS01/> ;
    skos:definition "Photosynthesizing microscopic protists and bacteria that inhabit the upper sunlit layer of marine and fresh water bodies."@en,
        "Non displonible"@fr ;
    skos:narrower <http://vocab.nerc.ac.uk/collection/A05/current/EV_PHYT/>,
        <https://gcos.wmo.int/en/essential-climate-variables/plankton> ;
    skos:notation "SDN:OD1::PHYTO" ;
    skos:note "accepted"@en ;
    skos:prefLabel "Phytoplankton"@en,
        "Phytoplancton"@fr .

<http://vocab.nerc.ac.uk/collection/OD1/current/PIGM/> a skos:Concept ;
    dc:identifier "SDN:OD1::PIGM" ;
    dcterms:date "2023-10-03 16:46:59.0" ;
    dcterms:identifier "SDN:OD1::PIGM" ;
    ns2:authoredOn "2023-10-03 16:46:59.0" ;
    ns2:hasCurrentVersion <http://vocab.nerc.ac.uk/collection/OD1/current/PIGM/2/> ;
    ns2:hasVersion <http://vocab.nerc.ac.uk/collection/OD1/current/PIGM/1/> ;
    ns2:version "2" ;
    void:inDataset <http://vocab.nerc.ac.uk/.well-known/void> ;
    owl:deprecated "false" ;
    owl:sameAs <http://vocab.nerc.ac.uk/collection/P03/current/B035/> ;
    owl:versionInfo "2" ;
    skos:altLabel "" ;
    skos:broader <http://vocab.nerc.ac.uk/collection/P02/current/CARO/>,
        <http://vocab.nerc.ac.uk/collection/P02/current/CPWC/>,
        <http://vocab.nerc.ac.uk/collection/P02/current/PHWC/>,
        <http://vocab.nerc.ac.uk/collection/P08/current/DS01/> ;
    skos:definition "Amount of photosynthetic pigments (chlorophyll, carotenoids, ...) in seawater using water column measurements."@en,
        "Non displonible"@fr ;
    skos:narrower <http://vocab.nerc.ac.uk/collection/A05/current/EV_CHLA/> ;
    skos:notation "SDN:OD1::PIGM" ;
    skos:note "accepted"@en ;
    skos:prefLabel "Pigments"@en,
        "Pigments"@fr .

<http://vocab.nerc.ac.uk/collection/OD1/current/PRESS/> a skos:Concept ;
    dc:identifier "SDN:OD1::PRESS" ;
    dcterms:date "2023-10-10 14:51:12.0" ;
    dcterms:identifier "SDN:OD1::PRESS" ;
    ns2:authoredOn "2023-10-10 14:51:12.0" ;
    ns2:hasCurrentVersion <http://vocab.nerc.ac.uk/collection/OD1/current/PRESS/1/> ;
    ns2:version "1" ;
    void:inDataset <http://vocab.nerc.ac.uk/.well-known/void> ;
    owl:deprecated "false" ;
    owl:versionInfo "1" ;
    skos:altLabel "" ;
    skos:broader <http://vocab.nerc.ac.uk/collection/P02/current/AHGT/>,
        <http://vocab.nerc.ac.uk/collection/P03/current/Z005/>,
        <http://vocab.nerc.ac.uk/collection/P08/current/DS07/> ;
    skos:definition "Depth below surface of the water body."@en,
        "Non displonible"@fr ;
    skos:notation "SDN:OD1::PRESS" ;
    skos:note "accepted"@en ;
    skos:prefLabel "Pressure"@en,
        "Pression"@fr .

<http://vocab.nerc.ac.uk/collection/OD1/current/RADFLX/> a skos:Concept ;
    dc:identifier "SDN:OD1::RADFLX" ;
    dcterms:date "2023-10-10 14:51:12.0" ;
    dcterms:identifier "SDN:OD1::RADFLX" ;
    ns2:authoredOn "2023-10-10 14:51:12.0" ;
    ns2:hasCurrentVersion <http://vocab.nerc.ac.uk/collection/OD1/current/RADFLX/1/> ;
    ns2:version "1" ;
    void:inDataset <http://vocab.nerc.ac.uk/.well-known/void> ;
    owl:deprecated "false" ;
    owl:sameAs <http://vocab.nerc.ac.uk/collection/A05/current/EV_RADFLX/> ;
    owl:versionInfo "1" ;
    skos:altLabel "" ;
    skos:broader <http://vocab.nerc.ac.uk/collection/P02/current/CSLR/>,
        <http://vocab.nerc.ac.uk/collection/P02/current/VSRA/>,
        <http://vocab.nerc.ac.uk/collection/P02/current/VSRW/>,
        <http://vocab.nerc.ac.uk/collection/P03/current/D015/>,
        <http://vocab.nerc.ac.uk/collection/P03/current/M010/>,
        <http://vocab.nerc.ac.uk/collection/P08/current/DS03/>,
        <http://vocab.nerc.ac.uk/collection/P08/current/DS05/> ;
    skos:definition "Variables associated with the determination of fluxes of radiation (downwelling and upwelling irradiance) in the atmosphere to and from the sea surface."@en,
        "Non displonible"@fr ;
    skos:narrower <https://gcos.wmo.int/en/essential-climate-variables/surface-radiation> ;
    skos:notation "SDN:OD1::RADFLX" ;
    skos:note "accepted"@en ;
    skos:prefLabel "Radiative flux"@en,
        "Flux radiatif"@fr .

<http://vocab.nerc.ac.uk/collection/OD1/current/RAIN/> a skos:Concept ;
    dc:identifier "SDN:OD1::RAIN" ;
    dcterms:date "2023-10-10 14:51:12.0" ;
    dcterms:identifier "SDN:OD1::RAIN" ;
    ns2:authoredOn "2023-10-10 14:51:12.0" ;
    ns2:hasCurrentVersion <http://vocab.nerc.ac.uk/collection/OD1/current/RAIN/1/> ;
    ns2:version "1" ;
    void:inDataset <http://vocab.nerc.ac.uk/.well-known/void> ;
    owl:deprecated "false" ;
    owl:sameAs <http://vocab.nerc.ac.uk/collection/A05/current/EV_RAIN/>,
        <http://vocab.nerc.ac.uk/collection/P02/current/CPRP/>,
        <http://vocab.nerc.ac.uk/collection/P02/current/RWCH/> ;
    owl:versionInfo "1" ;
    skos:altLabel "" ;
    skos:broader <http://vocab.nerc.ac.uk/collection/P03/current/M005/>,
        <http://vocab.nerc.ac.uk/collection/P03/current/M010/>,
        <http://vocab.nerc.ac.uk/collection/P08/current/DS05/> ;
    skos:definition "Variables associated with the determination of the amount of liquid and solid precipitations on the Earth's surface"@en,
        "Non displonible"@fr ;
    skos:narrower <https://gcos.wmo.int/en/essential-climate-variables/precipitation> ;
    skos:notation "SDN:OD1::RAIN" ;
    skos:note "accepted"@en ;
    skos:prefLabel "Rain"@en,
        "Pluviométrie"@fr .

<http://vocab.nerc.ac.uk/collection/OD1/current/SAL/> a skos:Concept ;
    dc:identifier "SDN:OD1::SAL" ;
    dcterms:date "2023-10-10 14:51:12.0" ;
    dcterms:identifier "SDN:OD1::SAL" ;
    ns2:authoredOn "2023-10-10 14:51:12.0" ;
    ns2:hasCurrentVersion <http://vocab.nerc.ac.uk/collection/OD1/current/SAL/1/> ;
    ns2:version "1" ;
    void:inDataset <http://vocab.nerc.ac.uk/.well-known/void> ;
    owl:deprecated "false" ;
    owl:sameAs <http://vocab.nerc.ac.uk/collection/A05/current/EV_SALIN/>,
        <http://vocab.nerc.ac.uk/collection/P02/current/PSAL/> ;
    owl:versionInfo "1" ;
    skos:altLabel "" ;
    skos:broader <http://vocab.nerc.ac.uk/collection/P03/current/D025/>,
        <http://vocab.nerc.ac.uk/collection/P08/current/DS03/> ;
    skos:definition "Variables associated with the determination of seawater salinity."@en,
        "Non displonible"@fr ;
    skos:notation "SDN:OD1::SAL" ;
    skos:note "accepted"@en ;
    skos:prefLabel "Salinity"@en,
        "Salinité"@fr .

<http://vocab.nerc.ac.uk/collection/OD1/current/SEAICE/> a skos:Concept ;
    dc:identifier "SDN:OD1::SEAICE" ;
    dcterms:date "2023-10-10 14:51:12.0" ;
    dcterms:identifier "SDN:OD1::SEAICE" ;
    ns2:authoredOn "2023-10-10 14:51:12.0" ;
    ns2:hasCurrentVersion <http://vocab.nerc.ac.uk/collection/OD1/current/SEAICE/1/> ;
    ns2:version "1" ;
    void:inDataset <http://vocab.nerc.ac.uk/.well-known/void> ;
    owl:deprecated "false" ;
    owl:sameAs <https://gcos.wmo.int/en/essential-climate-variables/sea-ice> ;
    owl:versionInfo "1" ;
    skos:altLabel "" ;
    skos:broader <http://vocab.nerc.ac.uk/collection/P02/current/ICEM/>,
        <http://vocab.nerc.ac.uk/collection/P02/current/IPHY/>,
        <http://vocab.nerc.ac.uk/collection/P03/current/M015/>,
        <http://vocab.nerc.ac.uk/collection/P08/current/DS09/> ;
    skos:definition "Variables associated with the determination of the amount and characterisation of sea ice."@en,
        "Non displonible"@fr ;
    skos:notation "SDN:OD1::SEAICE" ;
    skos:note "accepted"@en ;
    skos:prefLabel "Sea ice"@en,
        "Glace de mer"@fr .

<http://vocab.nerc.ac.uk/collection/OD1/current/SEALVL/> a skos:Concept ;
    dc:identifier "SDN:OD1::SEALVL" ;
    dcterms:date "2023-10-10 14:51:12.0" ;
    dcterms:identifier "SDN:OD1::SEALVL" ;
    ns2:authoredOn "2023-10-10 14:51:12.0" ;
    ns2:hasCurrentVersion <http://vocab.nerc.ac.uk/collection/OD1/current/SEALVL/1/> ;
    ns2:version "1" ;
    void:inDataset <http://vocab.nerc.ac.uk/.well-known/void> ;
    owl:deprecated "false" ;
    owl:sameAs <http://vocab.nerc.ac.uk/collection/A05/current/EV_SEALVL/> ;
    owl:versionInfo "1" ;
    skos:altLabel "" ;
    skos:broader <http://vocab.nerc.ac.uk/collection/P02/current/ASLV/>,
        <http://vocab.nerc.ac.uk/collection/P03/current/D032/>,
        <http://vocab.nerc.ac.uk/collection/P08/current/DS03/> ;
    skos:definition "The displacement of the water column surface from a fixed, stable reference, expressed as metres or pressure."@en,
        "Non displonible"@fr ;
    skos:notation "SDN:OD1::SEALVL" ;
    skos:note "accepted"@en ;
    skos:prefLabel "Sea surface height"@en,
        "Hauteur de la surface de la mer"@fr .

<http://vocab.nerc.ac.uk/collection/OD1/current/SEATEMP/> a skos:Concept ;
    dc:identifier "SDN:OD1::SEATEMP" ;
    dcterms:date "2023-10-10 14:51:12.0" ;
    dcterms:identifier "SDN:OD1::SEATEMP" ;
    ns2:authoredOn "2023-10-10 14:51:12.0" ;
    ns2:hasCurrentVersion <http://vocab.nerc.ac.uk/collection/OD1/current/SEATEMP/1/> ;
    ns2:version "1" ;
    void:inDataset <http://vocab.nerc.ac.uk/.well-known/void> ;
    owl:deprecated "false" ;
    owl:sameAs <http://vocab.nerc.ac.uk/collection/A05/current/EV_SEATEMP/>,
        <http://vocab.nerc.ac.uk/collection/P02/current/TEMP/> ;
    owl:versionInfo "1" ;
    skos:altLabel "" ;
    skos:broader <http://vocab.nerc.ac.uk/collection/P03/current/D025/>,
        <http://vocab.nerc.ac.uk/collection/P08/current/DS03/> ;
    skos:definition "Variables associated with the determination of seawater temperature."@en,
        "Non displonible"@fr ;
    skos:notation "SDN:OD1::SEATEMP" ;
    skos:note "accepted"@en ;
    skos:prefLabel "Sea temperature"@en,
        "Température de la mer"@fr .

<http://vocab.nerc.ac.uk/collection/OD1/current/SEDFLUX/> a skos:Concept ;
    dc:identifier "SDN:OD1::SEDFLUX" ;
    dcterms:date "2023-10-03 16:46:59.0" ;
    dcterms:identifier "SDN:OD1::SEDFLUX" ;
    ns2:authoredOn "2023-10-03 16:46:59.0" ;
    ns2:hasCurrentVersion <http://vocab.nerc.ac.uk/collection/OD1/current/SEDFLUX/2/> ;
    ns2:hasVersion <http://vocab.nerc.ac.uk/collection/OD1/current/SEDFLUX/1/> ;
    ns2:version "2" ;
    void:inDataset <http://vocab.nerc.ac.uk/.well-known/void> ;
    owl:deprecated "false" ;
    owl:versionInfo "2" ;
    skos:altLabel "" ;
    skos:broader <http://vocab.nerc.ac.uk/collection/P03/current/O005/>,
        <http://vocab.nerc.ac.uk/collection/P08/current/DS06/> ;
    skos:definition "Settling flux of particles (inorganic species, biological detritus, pigments, carbon, ...) in the water column."@en,
        "Non displonible"@fr ;
    skos:notation "SDN:OD1::SEDFLUX" ;
    skos:note "accepted"@en ;
    skos:prefLabel "Sedimentary fluxes"@en,
        "Flux sédimentaires"@fr .

<http://vocab.nerc.ac.uk/collection/OD1/current/SEISM/> a skos:Concept ;
    dc:identifier "SDN:OD1::SEISM" ;
    dcterms:date "2024-06-06 16:49:45.0" ;
    dcterms:identifier "SDN:OD1::SEISM" ;
    ns2:authoredOn "2024-06-06 16:49:45.0" ;
    ns2:hasCurrentVersion <http://vocab.nerc.ac.uk/collection/OD1/current/SEISM/1/> ;
    ns2:version "1" ;
    void:inDataset <http://vocab.nerc.ac.uk/.well-known/void> ;
    owl:deprecated "false" ;
    owl:sameAs <http://vocab.nerc.ac.uk/collection/P03/current/G012/> ;
    owl:versionInfo "1" ;
    skos:altLabel "" ;
    skos:broader <http://vocab.nerc.ac.uk/collection/P08/current/DS04/> ;
    skos:definition "Parameters associated with determination of sub-floor structure based on the propogation of acoustic energy and acoustic imaging of the sea floor."@en,
        "Non displonible"@fr ;
    skos:notation "SDN:OD1::SEISM" ;
    skos:note "accepted"@en ;
    skos:prefLabel "Seismic"@en,
        "Sismique"@fr .

<http://vocab.nerc.ac.uk/collection/OD1/current/SGRAS/> a skos:Concept ;
    dc:identifier "SDN:OD1::SGRAS" ;
    dcterms:date "2024-06-06 16:49:45.0" ;
    dcterms:identifier "SDN:OD1::SGRAS" ;
    ns2:authoredOn "2024-06-06 16:49:45.0" ;
    ns2:hasCurrentVersion <http://vocab.nerc.ac.uk/collection/OD1/current/SGRAS/1/> ;
    ns2:version "1" ;
    void:inDataset <http://vocab.nerc.ac.uk/.well-known/void> ;
    owl:deprecated "false" ;
    owl:sameAs <http://vocab.nerc.ac.uk/collection/P03/current/B055/> ;
    owl:versionInfo "1" ;
    skos:altLabel "" ;
    skos:broader <http://vocab.nerc.ac.uk/collection/P08/current/DS01/> ;
    skos:definition "Parameters pertaining to seagrass."@en,
        "Non displonible"@fr ;
    skos:notation "SDN:OD1::SGRAS" ;
    skos:note "accepted"@en ;
    skos:prefLabel "Seagrass"@en,
        "Herbiers"@fr .

<http://vocab.nerc.ac.uk/collection/OD1/current/SHORE/> a skos:Concept ;
    dc:identifier "SDN:OD1::SHORE" ;
    dcterms:date "2023-09-28 13:57:47.0" ;
    dcterms:identifier "SDN:OD1::SHORE" ;
    ns2:authoredOn "2023-09-28 13:57:47.0" ;
    ns2:hasCurrentVersion <http://vocab.nerc.ac.uk/collection/OD1/current/SHORE/1/> ;
    ns2:version "1" ;
    void:inDataset <http://vocab.nerc.ac.uk/.well-known/void> ;
    owl:deprecated "false" ;
    owl:sameAs <http://vocab.nerc.ac.uk/collection/P02/current/COGE/> ;
    owl:versionInfo "1" ;
    skos:altLabel "" ;
    skos:broader <http://vocab.nerc.ac.uk/collection/P03/current/GMAR/>,
        <http://vocab.nerc.ac.uk/collection/P08/current/DS04/> ;
    skos:definition "The distance over which the coast has moved due to a combination of factors; i.e., sea level rise, erosion, or sedimentation."@en,
        "Non displonible"@fr ;
    skos:notation "SDN:OD1::SHORE" ;
    skos:note "accepted"@en ;
    skos:prefLabel "Shoreline"@en,
        "Trait de côte"@fr .

<http://vocab.nerc.ac.uk/collection/OD1/current/SUSPMA/> a skos:Concept ;
    dc:identifier "SDN:OD1::SUSPMA" ;
    dcterms:date "2023-09-28 13:57:47.0" ;
    dcterms:identifier "SDN:OD1::SUSPMA" ;
    ns2:authoredOn "2023-09-28 13:57:47.0" ;
    ns2:hasCurrentVersion <http://vocab.nerc.ac.uk/collection/OD1/current/SUSPMA/1/> ;
    ns2:version "1" ;
    void:inDataset <http://vocab.nerc.ac.uk/.well-known/void> ;
    owl:deprecated "false" ;
    owl:sameAs <http://vocab.nerc.ac.uk/collection/P03/current/G015/> ;
    owl:versionInfo "1" ;
    skos:altLabel "" ;
    skos:broader <http://vocab.nerc.ac.uk/collection/P08/current/DS04/> ;
    skos:definition "Amount of particulate organic matter (turbidity) in seawater using water column measurements."@en,
        "Non displonible"@fr ;
    skos:narrower <http://vocab.nerc.ac.uk/collection/A05/current/EV_POM/> ;
    skos:notation "SDN:OD1::SUSPMA" ;
    skos:note "accepted"@en ;
    skos:prefLabel "Suspended matter"@en,
        "Matières en suspension"@fr .

<http://vocab.nerc.ac.uk/collection/OD1/current/TIDES/> a skos:Concept ;
    dc:identifier "SDN:OD1::TIDES" ;
    dcterms:date "2023-10-22 17:27:16.0" ;
    dcterms:identifier "SDN:OD1::TIDES" ;
    ns2:authoredOn "2023-10-22 17:27:16.0" ;
    ns2:hasCurrentVersion <http://vocab.nerc.ac.uk/collection/OD1/current/TIDES/2/> ;
    ns2:hasVersion <http://vocab.nerc.ac.uk/collection/OD1/current/TIDES/1/> ;
    ns2:version "2" ;
    void:inDataset <http://vocab.nerc.ac.uk/.well-known/void> ;
    owl:deprecated "false" ;
    owl:versionInfo "2" ;
    skos:altLabel "" ;
    skos:broader <http://vocab.nerc.ac.uk/collection/P02/current/ASLV/>,
        <http://vocab.nerc.ac.uk/collection/P03/current/D032/>,
        <http://vocab.nerc.ac.uk/collection/P08/current/DS03/> ;
    skos:definition "Multi-period movement of sea level, the main part of which is the astronomical tide, due to the gravitational attraction of the sun and moon on the rotating earth."@en,
        "Non displonible"@fr ;
    skos:notation "SDN:OD1::TIDES" ;
    skos:note "accepted"@en ;
    skos:prefLabel "Tides"@en,
        "Marées"@fr .

<http://vocab.nerc.ac.uk/collection/OD1/current/TRACELE/> a skos:Concept ;
    dc:identifier "SDN:OD1::TRACELE" ;
    dcterms:date "2023-09-28 13:57:47.0" ;
    dcterms:identifier "SDN:OD1::TRACELE" ;
    ns2:authoredOn "2023-09-28 13:57:47.0" ;
    ns2:hasCurrentVersion <http://vocab.nerc.ac.uk/collection/OD1/current/TRACELE/1/> ;
    ns2:version "1" ;
    void:inDataset <http://vocab.nerc.ac.uk/.well-known/void> ;
    owl:deprecated "false" ;
    owl:sameAs <http://vocab.nerc.ac.uk/collection/P03/current/C030/> ;
    owl:versionInfo "1" ;
    skos:altLabel "" ;
    skos:broader <http://vocab.nerc.ac.uk/collection/P02/current/IRBO/>,
        <http://vocab.nerc.ac.uk/collection/P02/current/WSTB/>,
        <http://vocab.nerc.ac.uk/collection/P08/current/DS02/> ;
    skos:definition "An element whose dissolved concentration is between 50 and 0.05 micromoles per kilogram. Most are metals and can be referred to as trace metals. Specific names of trace elements may be entered as Detailed Variables"@en,
        "Non displonible"@fr ;
    skos:notation "SDN:OD1::TRACELE" ;
    skos:note "accepted"@en ;
    skos:prefLabel "Trace elements and their isotopes"@en,
        "Eléments trace et leurs isotopes"@fr .

<http://vocab.nerc.ac.uk/collection/OD1/current/TRANST/> a skos:Concept ;
    dc:identifier "SDN:OD1::TRANST" ;
    dcterms:date "2023-09-28 13:57:47.0" ;
    dcterms:identifier "SDN:OD1::TRANST" ;
    ns2:authoredOn "2023-09-28 13:57:47.0" ;
    ns2:hasCurrentVersion <http://vocab.nerc.ac.uk/collection/OD1/current/TRANST/1/> ;
    ns2:version "1" ;
    void:inDataset <http://vocab.nerc.ac.uk/.well-known/void> ;
    owl:deprecated "false" ;
    owl:sameAs <http://vocab.nerc.ac.uk/collection/A05/current/EV_TTRACE/>,
        <http://vocab.nerc.ac.uk/collection/P02/current/WCTR/>,
        <https://gcos.wmo.int/en/essential-climate-variables/transient-tracers> ;
    owl:versionInfo "1" ;
    skos:altLabel "" ;
    skos:broader <http://vocab.nerc.ac.uk/collection/P03/current/D020/>,
        <http://vocab.nerc.ac.uk/collection/P08/current/DS03/> ;
    skos:definition "Transient tracers are man-made chemical compounds released to the atmosphere at known quantities that can be used in the ocean to quantify ventilation, transit time distribution and transport time-scales. Measurement of transient tracers in the subsurface ocean thus provides information on the time-scales since the ocean was ventilated, i.e. in contact with the atmosphere. A combination of these tracers provide the means to constrain the transit time distribution (TTD) of a water-mass that allows inference of concentrations or fates of other transient compounds, such as anthropogenic carbon or nitrous oxide"@en,
        "Non displonible"@fr ;
    skos:notation "SDN:OD1::TRANST" ;
    skos:note "accepted"@en ;
    skos:prefLabel "Transient tracers"@en,
        "Traceurs transitoires"@fr .

<http://vocab.nerc.ac.uk/collection/OD1/current/TURBID/> a skos:Concept ;
    dc:identifier "SDN:OD1::TURBID" ;
    dcterms:date "2023-09-28 13:57:47.0" ;
    dcterms:identifier "SDN:OD1::TURBID" ;
    ns2:authoredOn "2023-09-28 13:57:47.0" ;
    ns2:hasCurrentVersion <http://vocab.nerc.ac.uk/collection/OD1/current/TURBID/1/> ;
    ns2:version "1" ;
    void:inDataset <http://vocab.nerc.ac.uk/.well-known/void> ;
    owl:deprecated "false" ;
    owl:sameAs <http://vocab.nerc.ac.uk/collection/P02/current/TSED/>,
        <http://vocab.nerc.ac.uk/collection/P02/current/TVLT/> ;
    owl:versionInfo "1" ;
    skos:altLabel "" ;
    skos:broader <http://vocab.nerc.ac.uk/collection/P03/current/D015/>,
        <http://vocab.nerc.ac.uk/collection/P03/current/G015/>,
        <http://vocab.nerc.ac.uk/collection/P08/current/DS03/>,
        <http://vocab.nerc.ac.uk/collection/P08/current/DS04/> ;
    skos:definition "Measurement of the degree of scattering of light in water, related to the amount of suspended material in the water."@en,
        "Non displonible"@fr ;
    skos:narrower <http://vocab.nerc.ac.uk/collection/A05/current/EV_POM/> ;
    skos:notation "SDN:OD1::TURBID" ;
    skos:note "accepted"@en ;
    skos:prefLabel "Turbidity"@en,
        "Turbidité"@fr .

<http://vocab.nerc.ac.uk/collection/OD1/current/WAVES/> a skos:Concept ;
    dc:identifier "SDN:OD1::WAVES" ;
    dcterms:date "2023-10-10 14:51:12.0" ;
    dcterms:identifier "SDN:OD1::WAVES" ;
    ns2:authoredOn "2023-10-10 14:51:12.0" ;
    ns2:hasCurrentVersion <http://vocab.nerc.ac.uk/collection/OD1/current/WAVES/1/> ;
    ns2:version "1" ;
    void:inDataset <http://vocab.nerc.ac.uk/.well-known/void> ;
    owl:deprecated "false" ;
    owl:sameAs <http://vocab.nerc.ac.uk/collection/A05/current/EV_WAVES/>,
        <http://vocab.nerc.ac.uk/collection/P03/current/D034/> ;
    owl:versionInfo "1" ;
    skos:altLabel "" ;
    skos:broader <http://vocab.nerc.ac.uk/collection/P08/current/DS03/> ;
    skos:definition "Variables associated with the determination of surface waves on water bodies."@en,
        "Non displonible"@fr ;
    skos:notation "SDN:OD1::WAVES" ;
    skos:note "accepted"@en ;
    skos:prefLabel "Waves"@en,
        "Vagues"@fr .

<http://vocab.nerc.ac.uk/collection/OD1/current/WIND/> a skos:Concept ;
    dc:identifier "SDN:OD1::WIND" ;
    dcterms:date "2023-10-10 14:51:12.0" ;
    dcterms:identifier "SDN:OD1::WIND" ;
    ns2:authoredOn "2023-10-10 14:51:12.0" ;
    ns2:hasCurrentVersion <http://vocab.nerc.ac.uk/collection/OD1/current/WIND/1/> ;
    ns2:version "1" ;
    void:inDataset <http://vocab.nerc.ac.uk/.well-known/void> ;
    owl:deprecated "false" ;
    owl:versionInfo "1" ;
    skos:altLabel "" ;
    skos:broader <http://vocab.nerc.ac.uk/collection/P02/current/EWSB/>,
        <http://vocab.nerc.ac.uk/collection/P02/current/WSTR/>,
        <http://vocab.nerc.ac.uk/collection/P03/current/M010/>,
        <http://vocab.nerc.ac.uk/collection/P08/current/DS05/> ;
    skos:definition "Variables associated with the determination of the wind speed and direction near the Earth's surface."@en,
        "Non displonible"@fr ;
    skos:narrower <http://vocab.nerc.ac.uk/collection/A05/current/EV_WDIR/> ;
    skos:notation "SDN:OD1::WIND" ;
    skos:note "accepted"@en ;
    skos:prefLabel "Wind"@en,
        "Vent"@fr .

<http://vocab.nerc.ac.uk/collection/OD1/current/ZOO/> a skos:Concept ;
    dc:identifier "SDN:OD1::ZOO" ;
    dcterms:date "2023-09-28 13:57:47.0" ;
    dcterms:identifier "SDN:OD1::ZOO" ;
    ns2:authoredOn "2023-09-28 13:57:47.0" ;
    ns2:hasCurrentVersion <http://vocab.nerc.ac.uk/collection/OD1/current/ZOO/1/> ;
    ns2:version "1" ;
    void:inDataset <http://vocab.nerc.ac.uk/.well-known/void> ;
    owl:deprecated "false" ;
    owl:sameAs <http://vocab.nerc.ac.uk/collection/P03/current/B045/> ;
    owl:versionInfo "1" ;
    skos:altLabel "" ;
    skos:broader <http://vocab.nerc.ac.uk/collection/P08/current/DS01/> ;
    skos:definition "Zooplankton is the animal portion of the plankton; the animal community in marine and freshwater situations that floats free in the water, independent of the shore and the bottom, incapable of overcoming the speed of the surrounding currents and therefore moving with them."@en,
        "Non displonible"@fr ;
    skos:narrower <http://vocab.nerc.ac.uk/collection/A05/current/EV_ZOO/>,
        <https://gcos.wmo.int/en/essential-climate-variables/plankton> ;
    skos:notation "SDN:OD1::ZOO" ;
    skos:note "accepted"@en ;
    skos:prefLabel "Zooplankton"@en,
        "Zooplancton"@fr .

<https://w3id.org/earthsemantics/ODATIS/IR> a skos:Concept ;
    rdfs:seeAlso <https://sextant.ifremer.fr/geonetwork/srv/api/registries/vocabularies/local.theme.IR> ;
    skos:inScheme base: ;
    skos:prefLabel "Research infrastructure"@en,
        "Infrastructure de recherche"@fr .

<https://w3id.org/earthsemantics/ODATIS/type_jeux_donnee> a skos:Concept ;
    rdfs:seeAlso <https://sextant.ifremer.fr/geonetwork/srv/api/registries/vocabularies/local.theme.type_jeux_donnee> ;
    skos:inScheme base: ;
    skos:prefLabel "Dataset type"@en,
        "Type de jeux de données"@fr .

<https://w3id.org/earthsemantics/ODATIS/odatis_centre_donnees> a skos:Concept ;
    rdfs:seeAlso <https://sextant.ifremer.fr/geonetwork/srv/api/registries/vocabularies/local.theme.odatis_centre_donnees> ;
    skos:inScheme base: ;
    skos:prefLabel "Data center"@en,
        "Centre de données"@fr .

<https://w3id.org/earthsemantics/ODATIS/SNO> a skos:Concept ;
    rdfs:seeAlso <https://sextant.ifremer.fr/geonetwork/srv/api/registries/vocabularies/local.theme.SNO> ;
    skos:inScheme base: ;
    skos:prefLabel "National service of observation"@en,
        "Service nationaux d'observation"@fr .

base: a owl:Ontology,
        skos:ConceptScheme ;
    rdfs:label "ODATIS thesaurus"@en,
        "Thésaurus ODATIS"@fr ;
    owl:imports <https://sextant.ifremer.fr/geonetwork/srv/api/registries/vocabularies/local.theme.IR>,
        <https://sextant.ifremer.fr/geonetwork/srv/api/registries/vocabularies/local.theme.SNO>,
        <https://sextant.ifremer.fr/geonetwork/srv/api/registries/vocabularies/local.theme.odatis_centre_donnees>,
        <https://sextant.ifremer.fr/geonetwork/srv/api/registries/vocabularies/local.theme.type_jeux_donnee> ;
    skos:hasTopConcept <https://w3id.org/earthsemantics/ODATIS/IR>,
        <https://w3id.org/earthsemantics/ODATIS/SNO>,
        <https://w3id.org/earthsemantics/ODATIS/odatis_centre_donnees>,
        <https://w3id.org/earthsemantics/ODATIS/type_jeux_donnee> .

